If you have a binomial expression of the form $(a + b)$, where $a$ and $b$ are any real numbers or algebraic expressions, then squaring this binomial means multiplying it by itself.

The square of $(a + b)$ can be found using the distributive property or by applying the formula for the square of a binomial:

$$(a + b)^2 = (a + b)(a + b)$$

Using the distributive property to multiply, we get:

$$
\begin{align*}
(a + b)(a + b) & = a(a + b) + b(a + b) \\ \\
& = a^2 + ab + ab + b^2 \\ \\
& = a^2 + 2ab + b^2 \\
\end{align*}
$$

So, $(a + b)^2 = a^2 + 2ab + b^2$.

