---
tags:
  - notes
---
 See also: [[Difference of Squares]]

Sure! The difference of squares can be very useful in trigonometry for simplifying expressions and solving equations that involve trigonometric functions. Hereâ€™s how you can apply it.

### Basic Concept

The difference of squares formula is:
\[ a^2 - b^2 = (a + b)(a - b) \]

In trigonometry, we often encounter expressions that can be written in the form of \( \sin^2(x) - \cos^2(x) \) or similar. These expressions can be factored using the difference of squares formula.

### Example 1: Simplifying Trigonometric Expressions

Consider the expression \( \sin^2(x) - \cos^2(x) \).

1. **Identify the squares**:
   - \( \sin^2(x) = (\sin(x))^2 \)
   - \( \cos^2(x) = (\cos(x))^2 \)

2. **Apply the difference of squares formula**:
   \[ \sin^2(x) - \cos^2(x) = (\sin(x) + \cos(x))(\sin(x) - \cos(x)) \]

This simplifies the trigonometric expression.

### Example 2: Solving Trigonometric Equations

Suppose we need to solve the equation \( \sin^2(x) - \cos^2(x) = 0 \).

1. **Rewrite using the difference of squares**:
   \[ \sin^2(x) - \cos^2(x) = (\sin(x) + \cos(x))(\sin(x) - \cos(x)) = 0 \]

2. **Set each factor to zero**:
   \[ \sin(x) + \cos(x) = 0 \]
   or
   \[ \sin(x) - \cos(x) = 0 \]

3. **Solve each equation separately**:

   - For \( \sin(x) + \cos(x) = 0 \):
     \[ \sin(x) = -\cos(x) \]
     Divide both sides by \(\cos(x)\):
     \[ \tan(x) = -1 \]
     The solutions are:
     \[ x = \frac{3\pi}{4} + n\pi \]

   - For \( \sin(x) - \cos(x) = 0 \):
     \[ \sin(x) = \cos(x) \]
     Divide both sides by \(\cos(x)\):
     \[ \tan(x) = 1 \]
     The solutions are:
     \[ x = \frac{\pi}{4} + n\pi \]

Combining the solutions, we get:
\[ x = \frac{3\pi}{4} + n\pi \quad \text{or} \quad x = \frac{\pi}{4} + n\pi \]

### Example 3: Using Pythagorean Identities

Another application is using the Pythagorean identities. For instance, given the identity:
\[ \sin^2(x) + \cos^2(x) = 1 \]

We can derive new identities using the difference of squares. For example:
\[ 1 - \cos^2(x) = \sin^2(x) \]
\[ 1 - \sin^2(x) = \cos^2(x) \]

Suppose we want to factor \( 1 - \cos^2(x) \):
\[ 1 - \cos^2(x) = (\sqrt{1} + \cos(x))(\sqrt{1} - \cos(x)) \]
\[ = (1 + \cos(x))(1 - \cos(x)) \]

Since \( 1 - \cos^2(x) = \sin^2(x) \), we can write:
\[ \sin^2(x) = (1 + \cos(x))(1 - \cos(x)) \]

### Practice Problem

Factor \( \sin^4(x) - \cos^4(x) \).

1. Recognize it as a difference of squares:
   \[ \sin^4(x) - \cos^4(x) = (\sin^2(x))^2 - (\cos^2(x))^2 \]

2. Apply the difference of squares formula:
   \[ (\sin^2(x))^2 - (\cos^2(x))^2 = (\sin^2(x) + \cos^2(x))(\sin^2(x) - \cos^2(x)) \]

3. Use the Pythagorean identity \( \sin^2(x) + \cos^2(x) = 1 \):
   \[ (\sin^2(x) + \cos^2(x))(\sin^2(x) - \cos^2(x)) = 1 \cdot (\sin^2(x) - \cos^2(x)) \]
   \[ = \sin^2(x) - \cos^2(x) \]

So,
\[ \sin^4(x) - \cos^4(x) = (\sin^2(x) + \cos^2(x))(\sin^2(x) - \cos^2(x)) = 1 \cdot (\sin^2(x) - \cos^2(x)) = \sin^2(x) - \cos^2(x) \]

Using the difference of squares in trigonometry helps simplify expressions and solve equations efficiently.
