Solve the following rational equation $\frac{\displaystyle 2x}{\displaystyle x+3} - \frac{\displaystyle x}{\displaystyle x-3} = \frac{\displaystyle -18}{\displaystyle x^2-9}$

> [!success]+ Solutions
> $$\frac{2x}{x+3} - \frac{x}{x-3} - \frac{-18}{(x-3)(x+3)} = 0$$
> $$\text{LCD: } (x-3)(x+3)$$
> $$2x(x-3) - x(x+3) - (-18) = 0$$
> $$2x^2-6x-x^2-3x+18=0$$
> $$x^2-9x+18=0$$
> $$(x-3)(x-6)=0$$
> $$x=3, 6, x\neq\pm3$$
$$x=3 \text{ is an extraneous root, so the only valid solution is } x=6, x\neq\pm3$$